semantics/proofs/compute_interpLib.sml
@@ -4,12 +4,15 @@ open HolKernel boolLib bossLib lcsymtacs bigStepTheory replTheory
   val add_datatype = compute_basicLib.add_datatype
   fun add_interp_compset compset = let
     local open interpTheory in
+      val () = compute_semanticsLib.add_ast_compset compset
+      
       val () = computeLib.add_thms
       [run_eval_def
       ,run_eval_dec_def
       ,run_eval_decs_def
       ,run_eval_top_def
       ,run_eval_prog_def
+      ,run_eval_whole_prog_def
       ,result_return_def
       ,result_bind_def
       ,result_raise_def
@@ -19,6 +22,7 @@ open HolKernel boolLib bossLib lcsymtacs bigStepTheory replTheory
       ,prog_to_mods_def
       ,no_dup_top_types_def
       ,prog_to_top_types_def
+      ,bigClockTheory.set_counter_def
       ] compset
     end
     in
@@ -27,8 +31,6 @@ open HolKernel boolLib bossLib lcsymtacs bigStepTheory replTheory
 
   val the_interp_compset = let
     val c = wordsLib.words_compset ()
-    val () = compute_basicLib.add_basic_compset c
-    val () = compute_semanticsLib.add_ast_compset c
     val () = add_interp_compset c
     in
       c
